testing/TestDep/testing/LocalDepWithLampeV2/lampe/LocalDepWithLampe-2.0.0/Extracted.lean
@@ -2,7 +2,9 @@
 
 import «LocalDepWithLampe-2.0.0».Extracted.GeneratedTypes
 import «LocalDepWithLampe-2.0.0».Extracted.Lib
+import «std-1.0.0-beta.12».Extracted
 
 namespace «LocalDepWithLampe-2.0.0»
 
 def env := Lib.env
+  ++ «std-1.0.0-beta.12».env
