testing/TestDep/lampe/TestDep-0.0.0.lean
@@ -2,3 +2,201 @@
 
 import «TestDep-0.0.0».Extracted
 
+open Lampe
+
+-- TODO: This is required by `enter_decl`, we should explore why and fix it
+set_option maxRecDepth 8192
+
+theorem t1 {lp}: STHoare lp «TestDep-0.0.0».env (⟦⟧)
+    («GitDep-0.0.0::hello».call h![] h![])
+      fun output => (String.mk output.toList) = "hello-git-dep" := by
+  enter_decl
+  steps []
+  subst_vars
+  rfl
+
+theorem t2 {lp}: STHoare lp «TestDep-0.0.0».env (⟦⟧)
+    («GitDep-0.0.0::hello_git_dep».call h![] h![])
+      fun output => (String.mk output.toList) = "hello-git-dep" := by
+  enter_decl
+  steps []
+  subst_vars
+  rfl
+
+theorem t3 {lp}: STHoare lp «TestDep-0.0.0».env (⟦⟧)
+    («GitDep-1.0.0::hello».call h![] h![])
+      fun output => (String.mk output.toList) = "hello-git-dep-v1" := by
+  enter_decl
+  steps []
+  subst_vars
+  rfl
+
+theorem t4 {lp}: STHoare lp «TestDep-0.0.0».env (⟦⟧)
+    («GitDep-1.0.0::hello_git_dep_v1».call h![] h![])
+      fun output => (String.mk output.toList) = "hello-git-dep-v1" := by
+  enter_decl
+  steps []
+  subst_vars
+  rfl
+
+theorem t5 {lp}: STHoare lp «TestDep-0.0.0».env (⟦⟧)
+    («GitDep-2.0.0::hello».call h![] h![])
+      fun output => (String.mk output.toList) = "hello-git-dep-v2" := by
+  enter_decl
+  steps []
+  subst_vars
+  rfl
+
+theorem t6 {lp}: STHoare lp «TestDep-0.0.0».env (⟦⟧)
+    («GitDep-2.0.0::hello_git_dep_v2».call h![] h![])
+      fun output => (String.mk output.toList) = "hello-git-dep-v2" := by
+  enter_decl
+  steps []
+  subst_vars
+  rfl
+
+theorem t11 {lp}: STHoare lp «TestDep-0.0.0».env (⟦⟧)
+    («LocalDep-0.0.0::hello».call h![] h![])
+      fun output => (String.mk output.toList) = "hello-local-dep" := by
+  enter_decl
+  steps []
+  subst_vars
+  rfl
+
+theorem t12 {lp}: STHoare lp «TestDep-0.0.0».env (⟦⟧)
+    («LocalDep-0.0.0::hello_local_dep».call h![] h![])
+      fun output => (String.mk output.toList) = "hello-local-dep" := by
+  enter_decl
+  steps []
+  subst_vars
+  rfl
+
+theorem t13 {lp}: STHoare lp «TestDep-0.0.0».env (⟦⟧)
+    («LocalDep-1.0.0::hello».call h![] h![])
+      fun output => (String.mk output.toList) = "hello-local-dep-v1" := by
+  enter_decl
+  steps []
+  subst_vars
+  rfl
+
+theorem t14 {lp}: STHoare lp «TestDep-0.0.0».env (⟦⟧)
+    («LocalDep-1.0.0::hello_local_dep_v1».call h![] h![])
+      fun output => (String.mk output.toList) = "hello-local-dep-v1" := by
+  enter_decl
+  steps []
+  subst_vars
+  rfl
+
+theorem t15 {lp}: STHoare lp «TestDep-0.0.0».env (⟦⟧)
+    («LocalDep-2.0.0::hello».call h![] h![])
+      fun output => (String.mk output.toList) = "hello-local-dep-v2" := by
+  enter_decl
+  steps []
+  subst_vars
+  rfl
+
+theorem t16 {lp}: STHoare lp «TestDep-0.0.0».env (⟦⟧)
+    («LocalDep-2.0.0::hello_local_dep_v2».call h![] h![])
+      fun output => (String.mk output.toList) = "hello-local-dep-v2" := by
+  enter_decl
+  steps []
+  subst_vars
+  rfl
+
+
+theorem t21 {lp}: STHoare lp «TestDep-0.0.0».env (⟦⟧)
+    («GitDepWithLampe-0.0.0::hello».call h![] h![])
+      fun output => (String.mk output.toList) = "hello-git-dep-with-lampe" := by
+  enter_decl
+  steps []
+  subst_vars
+  rfl
+
+theorem t22 {lp}: STHoare lp «TestDep-0.0.0».env (⟦⟧)
+    («GitDepWithLampe-0.0.0::hello_git_dep_with_lampe».call h![] h![])
+      fun output => (String.mk output.toList) = "hello-git-dep-with-lampe" := by
+  enter_decl
+  steps []
+  subst_vars
+  rfl
+
+theorem t23 {lp}: STHoare lp «TestDep-0.0.0».env (⟦⟧)
+    («GitDepWithLampe-1.0.0::hello».call h![] h![])
+      fun output => (String.mk output.toList) = "hello-git-dep-with-lampe-v1" := by
+  enter_decl
+  steps []
+  subst_vars
+  rfl
+
+theorem t24 {lp}: STHoare lp «TestDep-0.0.0».env (⟦⟧)
+    («GitDepWithLampe-1.0.0::hello_git_dep_with_lampe_v1».call h![] h![])
+      fun output => (String.mk output.toList) = "hello-git-dep-with-lampe-v1" := by
+  enter_decl
+  steps []
+  subst_vars
+  rfl
+
+theorem t25 {lp}: STHoare lp «TestDep-0.0.0».env (⟦⟧)
+    («GitDepWithLampe-2.0.0::hello».call h![] h![])
+      fun output => (String.mk output.toList) = "hello-git-dep-with-lampe-v2" := by
+  enter_decl
+  steps []
+  subst_vars
+  rfl
+
+theorem t26 {lp}: STHoare lp «TestDep-0.0.0».env (⟦⟧)
+    («GitDepWithLampe-2.0.0::hello_git_dep_with_lampe_v2».call h![] h![])
+      fun output => (String.mk output.toList) = "hello-git-dep-with-lampe-v2" := by
+  enter_decl
+  steps []
+  subst_vars
+  rfl
+
+
+theorem t31 {lp}: STHoare lp «TestDep-0.0.0».env (⟦⟧)
+    («LocalDepWithLampe-0.0.0::hello».call h![] h![])
+      fun output => (String.mk output.toList) = "hello-local-dep-with-lampe" := by
+  enter_decl
+  steps []
+  subst_vars
+  rfl
+
+theorem t32 {lp}: STHoare lp «TestDep-0.0.0».env (⟦⟧)
+    («LocalDepWithLampe-0.0.0::hello_local_dep_with_lampe».call h![] h![])
+      fun output => (String.mk output.toList) = "hello-local-dep-with-lampe" := by
+  enter_decl
+  steps []
+  subst_vars
+  rfl
+
+theorem t33 {lp}: STHoare lp «TestDep-0.0.0».env (⟦⟧)
+    («LocalDepWithLampe-1.0.0::hello».call h![] h![])
+      fun output => (String.mk output.toList) = "hello-local-dep-with-lampe-v1" := by
+  enter_decl
+  steps []
+  subst_vars
+  rfl
+
+theorem t34 {lp}: STHoare lp «TestDep-0.0.0».env (⟦⟧)
+    («LocalDepWithLampe-1.0.0::hello_local_dep_with_lampe_v1».call h![] h![])
+      fun output => (String.mk output.toList) = "hello-local-dep-with-lampe-v1" := by
+  enter_decl
+  steps []
+  subst_vars
+  rfl
+
+theorem t35 {lp}: STHoare lp «TestDep-0.0.0».env (⟦⟧)
+    («LocalDepWithLampe-2.0.0::hello».call h![] h![])
+      fun output => (String.mk output.toList) = "hello-local-dep-with-lampe-v2" := by
+  enter_decl
+  steps []
+  subst_vars
+  rfl
+
+theorem t36 {lp}: STHoare lp «TestDep-0.0.0».env (⟦⟧)
+    («LocalDepWithLampe-2.0.0::hello_local_dep_with_lampe_v2».call h![] h![])
+      fun output => (String.mk output.toList) = "hello-local-dep-with-lampe-v2" := by
+  enter_decl
+  steps []
+  subst_vars
+  rfl
